spectec/test-coq/theories/type_preservation.v
@@ -2281,14 +2281,15 @@ Admitted.
 		remember (fun_invsigned 32 (0 - 1)%coq_nat) as v_n'.
 		eapply (Admin_instr_ok__instr _ _ (instr__CONST (valtype__INN inn__I32) v_n') (functype__ [] [(valtype__INN inn__I32)])).
 		apply Instr_ok__const.
-Qed.
+Qed. *)
 
 (* Ultimate goal of project *)				
 Theorem t_preservation: forall c1 ts c2,
 	Step c1 c2 ->
 	Config_ok c1 ts ->
 	Config_ok c2 ts.
-Proof.
+Admitted.
+(* Proof.
 	move => c1 ts c2 HReduce HType.
 	destruct c1; destruct v_state as [store1 frame1].
 	destruct c2; destruct v_state as [store2 frame2].
